NArith instead of ZArith

examples/homogeneous/Homogeneous.v
@@ -1,20 +1,21 @@
-Require Import ZArith.
-Open Scope Z_scope.
+Require Import NArith.
+Open Scope N_scope.
 
 Definition UINT_MIN := 0.
 Definition UINT_MAX := 2 ^ 256.
-Definition range (n : Z) := ((UINT_MIN <=? n) && (n <? UINT_MAX)) % bool.
+Definition range (n : N) := ((UINT_MIN <=? n) && (n <=? UINT_MAX)) % bool.
 
 Record State : Set :=
   state {
-      x : Z ;
-      y : Z ;
-      z : Z ;
+      x : N ;
+      y : N ;
+      z : N ;
     }.
 
+Check state.
 Definition BASE := state 3 5 15.
 
-Definition f (s : State) (scalar : Z) :=
+Definition f (s : State) (scalar : N) :=
   let x := x s in
   let y := y s in
   let z := z s in
@@ -23,7 +24,7 @@ Definition f (s : State) (scalar : Z) :=
   | _ , _ => s
   end.
 
-Definition g (s : State) (scalar : Z) :=
+Definition g (s : State) (scalar : N) :=
   let x := x s in
   let y := y s in
   let z := z s in
@@ -34,6 +35,6 @@ Definition g (s : State) (scalar : Z) :=
 
 Inductive reachable : State -> Prop :=
 | base : reachable BASE
-| f_step : forall (s : State) (scalar : Z), reachable s -> reachable (f s scalar)
-| g_step : forall (s : State) (scalar : Z), reachable s -> reachable (g s scalar)
+| f_step : forall (s : State) (scalar : N), reachable s -> reachable (f s scalar)
+| g_step : forall (s : State) (scalar : N), reachable s -> reachable (g s scalar)
 .
